SystemFD/Evaluator/Soundness.lean
@@ -4,32 +4,41 @@ import SystemFD.Ctx
 import SystemFD.Evaluator
 import SystemFD.Algorithm
 import SystemFD.Judgment
+set_option maxHeartbeats 500000
+
+
+theorem unfolding_eval_inst_lemma :
+   t.neutral_form = .some (h, sp) ->
+   eval_inst Γ t = (match (Γ d@ h) with
+                   | .openm _ =>
+                       List.map (·.apply_spine sp) (get_instances Γ (instance_indices' Γ 0 h []))
+                   | .term _ b => .some [ b.apply_spine sp ]  -- inline a let bound term
+                   | _ => .none) := by
+intros ih;
+sorry
 
 theorem eval_inst_soundess : eval_inst Γ t = .some ts -> Red Γ t ts := by
 intros
 induction Γ, t using eval_inst.induct generalizing ts
 case _ t Γ n sp tne a oa et =>
-  have tnf := Term.spine_lemma tne; subst tnf;
-  induction sp
-  case _ => simp_all; sorry
-  case _ => simp_all; sorry
+  have tnf := Term.spine_lemma tne; rw [tnf] at et;
+  simp_all; have uf := @unfolding_eval_inst_lemma Γ ((#n).apply_spine sp) n sp tne;
+  simp_all; rw[<-et];
+  generalize ip : instance_indices' Γ 0 n [] = i at *;
+  generalize instsp : get_instances Γ i = insts at *;
+  symm at instsp; symm at ip;
+  apply Red.inst tne _ ip instsp; rfl; simp_all;
 case _ t Γ n sp head A t' f et =>
-    have t' := Term.spine_lemma head; subst t'
-    symm at f; sorry
-    -- induction sp
-    --   case _ =>
-    --     have t' := Term.spine_lemma head; symm at head;
-    --     simp at t'; subst t'; simp at et; rw [f] at et; simp at et; symm at et; subst et;
-    --     symm at f; apply Red.letterm head f; rfl
-    --   case _ =>
-    --     have t' := Term.spine_lemma head; symm at head;
-    --     subst t'; rw [f] at et; simp at et; symm at et; subst et;
-    --     symm at f; apply Red.letterm head f; rfl
-
+    have t' := Term.spine_lemma head; subst t'; simp_all;
+    symm at f; have uf := @unfolding_eval_inst_lemma Γ ((#n).apply_spine sp) n sp head;
+    rw [uf] at et; simp_all; split at et;
+    case _ => simp_all
+    case _ a b heq => simp_all; symm at heq; rw [<-et]; apply Red.letterm head heq
+    case _ => simp_all
 case _ t Γ n sp head no nt et =>
   have t' := Term.spine_lemma head; subst t';
-  simp_all;
-  sorry
+  simp_all; have uf := @unfolding_eval_inst_lemma Γ ((#n).apply_spine sp) n sp head;
+  rw [uf] at et; simp_all
 case _ Γ a b f _ et => simp at et; subst et; apply Red.beta
 case _ Γ a b et => simp at et; subst et; apply Red.betat
 case _ Γ f t _ nf ih et =>
@@ -47,44 +56,118 @@ case _ nf ih et =>
     injection (And.right h) with ts; subst ts;
     apply Red.appt_congr ih'; rfl
 
+-- ITE
 case _ Γ p s b c _ ih et =>
   simp at et;
   rw[Option.bind_eq_some] at et;
   cases et; case _ w h =>
-  have pne := And.left h;
-  have smatch := And.right h;
-  simp at smatch;
-  sorry
+    have pne := And.left h;
+    have site := And.right h;
+    simp at site; split at site; simp_all;
+    case _ =>
+      rw[Option.bind_eq_some] at site;
+      cases site; case _ w h =>
+      injection (And.right h) with ts; subst ts;
+      apply Red.ite_congr (@ih w (And.left h)); trivial
+    case _ =>
+        simp_all; split at site;
+        case _ =>
+          simp_all; rw[Option.bind_eq_some] at site;
+          cases site; case _ w h =>
+            injection (And.right h) with ts; subst ts;
+            apply Red.ite_congr (@ih w (And.left h)); trivial
+        case _ sp' heq _ _ =>
+          simp at site; split at site;
+          case _ =>
+            simp_all; rw[Option.bind_eq_some] at site;
+            cases site; case _ w h =>
+            injection (And.right h) with ts; subst ts;
+            apply Red.ite_congr (@ih w (And.left h)); trivial
+          case _ =>
+            simp at site; split at site;
+            case _ ctor =>
+              simp at site; split at site;
+              case _  _ _ _ _ _ heq' =>
+                simp_all; have ss := And.right site; rw[<-ss]; symm at pne; symm at heq; symm at heq'
+                have ss' := And.left site; subst ss'; symm at ctor;
+                subst ss; simp_all; apply Red.ite_matched pne heq heq'; unfold Term.is_ctorid;
+                rw[<-ctor]
+              case _ cond =>
+                symm at heq; symm at pne;
+                have ss := And.left site; have ss' := And.right site; injection ss' with sss'; subst sss'
+                simp_all; apply Red.ite_missed pne heq;
+                have tt := option_neg cond; simp_all
+            case _ => simp at site
+
+-- GUARD
 case _ Γ p s c _ ih et =>
   simp at et;
   rw[Option.bind_eq_some] at et;
   cases et; case _ w h =>
   have pne := And.left h;
   have smatch := And.right h;
-  simp_all;
-  sorry
-case _ Γ _ _ ih => simp at ih; rw[<-ih]; apply Red.sym
-case _ ih η =>
-  simp at η; rw[Option.bind_eq_some] at η
-  cases η; case _ w η' =>
-    have ih' := @ih w (And.left η');
-    injection (And.right η') with ts'; symm at ts'; subst ts';
-    apply Red.sym_congr ih'; rfl
+  simp_all; split at smatch;
+  case _ =>
+    rw[Option.bind_eq_some] at smatch;
+    cases smatch; case _ s' smatch' =>
+    have ih' := @ih s' (And.left smatch'); simp_all
+    have h' := And.right smatch'; subst h'; apply Red.guard_congr ih'; rfl
+  case _ s' sp' heq =>
+    split at smatch;
+    case _ frame_term =>
+      simp_all; rw[Option.bind_eq_some] at smatch;
+      symm at heq; symm at frame_term; simp_all
+      cases smatch;
+      case _ w ts' =>
+        have ih' := @ih w (And.left ts'); simp_all
+        have h' := And.right ts'; subst h'; apply Red.guard_congr ih'; rfl
+    case _ =>
+      simp_all; split at smatch;
+      case _ =>
+        simp_all; rw[Option.bind_eq_some] at smatch; cases smatch;
+        case _ w ts' =>
+        have ih' := @ih w (And.left ts'); simp_all
+        have h' := And.right ts'; subst h'; apply Red.guard_congr ih'; rfl
+      case _ =>
+        simp_all; split at smatch;
+        case _ heq' => -- guard_matched
+             split at smatch;
+             case _ _ _ sl =>
+               injection smatch with smatch'; rw[<-smatch'];
+               symm at pne; symm at heq; symm at sl; rw [<-heq'] at heq;
+               apply Red.guard_matched pne heq sl
+             case _ x =>
+               symm at pne; symm at heq;
+               injection smatch with empt; subst empt
+               have temp := option_neg x;
+               simp_all; apply Red.guard_missed pne heq;
+               simp_all;
+        case _ c => -- guard_missed
+          simp_all; subst smatch; symm at pne; symm at heq;
+          apply Red.guard_missed pne heq;
+          simp_all;
 
-case _ Γ t t' teq nf ih =>
+case _ Γ _ _ et => simp at et; rw[<-et]; apply Red.sym
+case _ ih et =>
+  simp at et; rw[Option.bind_eq_some] at et;
+  cases et; case _ w h =>
+  have et' := ih (And.left h); simp_all; rw[<-And.right h];
+  apply Red.sym_congr et'; rfl
+
+case _ Γ t t' teq nf et =>
   have e := eq_of_beq teq; subst e;
-  simp at ih; rw [<-ih]; exact Red.seq
-case _ Γ t' t h x ih =>
-  simp at ih; have nh := And.left ih; exfalso;
+  simp at et; rw [<-et]; exact Red.seq
+case _ Γ t' t h x et =>
+  simp at et; have nh := And.left et; exfalso;
   contradiction
-case _ Γ t t' t'' teq x et=>
+case _ Γ t t' t'' teq _ et =>
   have eq := eq_of_beq teq; subst eq;
   simp at et; rw[<-et]; exact Red.appc
-case _ Γ t t' t'' teq x et=>
+case _ Γ t t' t'' teq x et =>
   simp at et; have nh := And.left et; contradiction
 
-case _ Γ A B _ et => simp at et; subst et; apply Red.fst
-case _ _ _ _ _ et => simp at et; subst et; apply Red.snd
+case _ et => simp at et; subst et; apply Red.fst
+case _ et => simp at et; subst et; apply Red.snd
 case _ et => simp at et; subst et; apply Red.arrowc
 case _ Γ t η _ _ ih et =>
   simp at et; rw[Option.bind_eq_some] at et;
