SystemFD/Util.lean
@@ -5,6 +5,14 @@ def prefix_equal [BEq T] : List T -> List T -> Option (List T)
 | .cons _ _, [] => .none
 | .cons x1 t1, .cons x2 t2 => if x1 == x2 then prefix_equal t1 t2 else .none
 
+
 instance : Monad List where -- This seems fishy. Why doesn't lean have a Monad List instance?
   pure a := List.cons a List.nil
   bind l f := List.flatMap l f
+
+
+theorem option_neg : (∀ l, ¬ (p = some l)) -> p = none := by
+  intros np;
+  cases p;
+  case _ => simp
+  case _ v => simp; exfalso; apply np v; rfl
